cryptis/core/term/base.v
@@ -144,6 +144,7 @@ elim/term_ind': t.
 - by move=> t IH.
 - by move=> pt w nf; exact: w.
 Qed.
+Hint Resolve wf_unfold_term : core.
 
 Lemma wf_unfold_terms ts : Forall (fun pt => PreTerm.wf pt) (unfold_term <$> ts).
 Proof.
@@ -232,23 +233,6 @@ Global Instance term_countable : Countable term :=
 Global Instance term_inhabited : Inhabited term.
 Proof. exact: (populate (TInt 0)). Qed.
 
-Definition term_order : relation term :=
-  fun t1 t2 => pt_order (unfold_term t1) (unfold_term t2).
-
-Global Instance term_order_dec : RelDecision term_order.
-Proof. rewrite /term_order => t1 t2; exact: pt_order_dec. Defined.
-Global Instance term_order_refl : Reflexive term_order.
-Proof. move=> t; apply: pt_order_refl. Qed.
-Global Instance term_order_trans : Transitive term_order.
-Proof. move=> x y z H1 H2; rewrite /term_order; eapply pt_order_trans; eassumption. Qed.
-Global Instance term_order_total : Total term_order.
-Proof. move=> x y; apply: pt_order_total. Qed.
-Global Instance term_order_antisymm : AntiSymm eq term_order.
-Proof.
-move=> x y H1 H2; apply: unfold_term_inj.
-by apply: (@anti_symm _ eq pt_order _).
-Qed.
-
 Canonical termO := leibnizO term.
 
 Global Instance aenc_key_eq_dec : EqDecision aenc_key.
@@ -296,28 +280,30 @@ Definition TExpN t ts := TExp t (TMulN ts).
 
 Lemma unfold_TInv t : unfold_term (TInv t) = PreTerm.inv (unfold_term t).
 Proof.
-by rewrite unlock unfold_fold
-  (PreTerm.normalize_wf _ (PreTerm.wf_inv _ (wf_unfold_term t))).
+rewrite unlock unfold_fold PreTerm.normalize_wf //.
+rewrite -(PreTerm.normalize_wf (unfold_term t)) //.
+apply: PreTerm.wf_inv.
+exact: PreTerm.wf_normalize.
 Qed.
 
 Lemma unfold_TExp b e :
   unfold_term (TExp b e) = PreTerm.exp (unfold_term b) (unfold_term e).
 Proof.
-by rewrite unlock unfold_fold
-  (PreTerm.normalize_wf _ (PreTerm.wf_exp _ _ (wf_unfold_term b) (wf_unfold_term e))).
+rewrite unlock unfold_fold PreTerm.normalize_wf //.
+rewrite -(PreTerm.normalize_wf (unfold_term b)) //.
+rewrite -(PreTerm.normalize_wf (unfold_term e)) //.
+apply: PreTerm.wf_exp.
+- exact: PreTerm.wf_normalize.
+- exact: PreTerm.wf_normalize.
 Qed.
 
 Lemma unfold_TMulN ts :
   unfold_term (TMulN ts) = PreTerm.mul (unfold_term <$> ts).
 Proof.
-by rewrite unlock unfold_fold
-  (PreTerm.normalize_wf _ (PreTerm.wf_mul _ (wf_unfold_terms ts))).
+rewrite unlock unfold_fold PreTerm.normalize_wf //.
+apply: PreTerm.wf_mul; rewrite Forall_fmap Forall_forall.
+by eauto.
 Qed.
-
-Lemma unfold_TExpN t ts :
-  unfold_term (TExpN t ts) =
-  PreTerm.exp (unfold_term t) (PreTerm.mul (unfold_term <$> ts)).
-Proof. by rewrite /TExpN unfold_TExp unfold_TMulN. Qed.
 
 Lemma fold_termE pt :
   fold_term pt =
@@ -344,7 +330,7 @@ case: pt => /=; try by case =>> //=; rewrite ?unfold_TInv !unfold_fold.
 Qed.
 
 Definition base t := fold_term (PreTerm.base (unfold_term t)).
-Definition exps t := fold_term <$> PreTerm.exps (unfold_term t).
+Definition expo t := fold_term (PreTerm.expo (unfold_term t)).
 Definition factors t := fold_term <$> PreTerm.factors (unfold_term t).
 
 Definition is_nonce t :=
@@ -371,162 +357,343 @@ Proof. by case: t. Qed.
 Lemma is_mul_unfold t : is_mul t = PreTerm.is_mul (unfold_term t).
 Proof. by case: t. Qed.
 
-Lemma unfold_TInv_Nmul {t} :
-  negb (is_mul t) -> unfold_term (TInv t) = PreTerm.inv_aux (unfold_term t).
-Proof.
-rewrite is_mul_unfold => Nm.
-by rewrite unfold_TInv (PreTerm.inv_Nmul _ Nm).
-Qed.
+Lemma unfold_base t : unfold_term (base t) = PreTerm.base (unfold_term t).
+Proof. rewrite /base fold_termK //; exact: PreTerm.wf_base. Qed.
 
-Lemma is_inv_TInv t : negb (is_mul t) -> is_inv (TInv t) = negb (is_inv t).
-Proof.
-move => Nm; rewrite !is_inv_unfold (unfold_TInv_Nmul Nm).
-move: (wf_unfold_term t); case: (unfold_term t) => [o|[k||] pt'|o t1 t2|ts] /= wf //.
-by move: wf => /andb_True [/andb_True [/negb_True/Is_true_false_1 -> _] _].
-Qed.
-
-Lemma is_exp_TInv t : negb (is_mul t) -> negb (is_inv t) -> negb (is_exp (TInv t)).
-Proof.
-move => Nm; rewrite is_inv_unfold => Ni.
-by rewrite is_exp_unfold (unfold_TInv_Nmul Nm) (PreTerm.inv_invN _ Ni).
-Qed.
-
-Lemma Nmul_TInv {t} : negb (is_mul t) -> negb (is_mul (TInv t)).
-Proof.
-move => Nm; rewrite is_mul_unfold (unfold_TInv_Nmul Nm).
-exact: (PreTerm.is_mul_inv_aux _ (wf_unfold_term t)).
-Qed.
+Lemma unfold_expo t : unfold_term (expo t) = PreTerm.expo (unfold_term t).
+Proof. rewrite /expo fold_termK //; exact: PreTerm.wf_expo. Qed.
 
 Lemma unfold_factors t :
   unfold_term <$> factors t = PreTerm.factors (unfold_term t).
 Proof.
-rewrite /factors fmap_fold_termK //.
-exact: (PreTerm.wf_factors _ (wf_unfold_term t)).
+rewrite /factors fmap_fold_termK //; apply/list.Forall_forall => t0 t0_in.
+apply: PreTerm.wf_factors_wf t0_in.
+exact: PreTerm.wf_wf_factors.
 Qed.
 
-Lemma count_factors_unfold {t} Y :
-  negb (is_mul t) ->
-  SMS.count TInv t (factors Y) =
-  SMS.count PreTerm.inv_aux (unfold_term t) (PreTerm.factors (unfold_term Y)).
+Lemma is_mulE t : is_mul t = bool_decide (length (factors t) ≠ 1).
 Proof.
-move=> Nt; rewrite -unfold_factors.
-by rewrite (SMS.count_fmap TInv PreTerm.inv_aux unfold_term t (factors Y)
-              (@unfold_term_inj) (unfold_TInv_Nmul Nt)).
+rewrite -(length_fmap unfold_term) unfold_factors is_mul_unfold.
+case: (unfold_term t) (wf_unfold_term t) => //= ts.
+by rewrite andb_True; case=> _ /Is_true_true ->.
 Qed.
 
-Lemma count_factors_TInv t t' :
-  negb (is_mul t) →
-  SMS.count TInv t (factors (TInv t')) = (- SMS.count TInv t (factors t'))%Z.
+Lemma is_inv_TInv t : negb (is_mul t) → is_inv (TInv t) = negb (is_inv t).
 Proof.
-move=> Nm; rewrite !count_factors_unfold // unfold_TInv.
-rewrite PreTerm.count_factors_inv //; exact: wf_unfold_term.
+rewrite !is_inv_unfold is_mul_unfold unfold_TInv.
+case: {t} (unfold_term t) (wf_unfold_term t) => //=.
+by case=> //= t; case: PreTerm.is_inv.
 Qed.
 
-Lemma count_factors_TMulN t t' ts :
-  negb (is_mul t) →
-  SMS.count TInv t (factors (TMulN (t' :: ts))) =
-  (SMS.count TInv t (factors t') + SMS.count TInv t (factors (TMulN ts)))%Z.
+Lemma is_exp_TInv t : negb (is_mul t) → negb (is_inv t) → negb (is_exp (TInv t)).
 Proof.
-move=> Nm.
-rewrite (count_factors_unfold (TMulN (t' :: ts)) Nm)
-        (count_factors_unfold t' Nm) (count_factors_unfold (TMulN ts) Nm)
-        !unfold_TMulN fmap_cons.
-exact: (PreTerm.count_factors_mul _ _ _
-          (wf_unfold_term t) (wf_unfold_term t') (wf_unfold_terms ts)).
+rewrite is_mul_unfold is_inv_unfold is_exp_unfold unfold_TInv.
+move=> Nm Ni; rewrite PreTerm.inv_Nmul //.
+case: (unfold_term t) Nm Ni => //=.
+by case=> //=.
 Qed.
 
-Lemma count_factors_inj t1 t2 :
-  (forall x, negb (is_mul x) ->
-     SMS.count TInv x (factors t1) = SMS.count TInv x (factors t2)) ->
+Lemma factors_inj t1 t2 : factors t1 = factors t2 → t1 = t2.
+Proof.
+move/(f_equal (λ ts : list _, unfold_term <$> ts)).
+rewrite !unfold_factors => e.
+apply: unfold_term_inj => /=.
+move: (unfold_term t2) (wf_unfold_term t2) => {}t2 wf2 in e *.
+move: (unfold_term t1) (wf_unfold_term t1) => {}t1 wf1 in e *.
+case: t1 t2 => [o1|o1 t1|o1 t11 t12|ts1] [o2|o2 t2|o2 t21 t22|ts2] //=
+  in wf1 wf2 e *;
+do 1?congruence.
+- by rewrite -e /= andb_false_r in wf2.
+- by rewrite -e /= andb_false_r in wf2.
+- by rewrite -e /= andb_false_r in wf2.
+- by rewrite e /= andb_false_r in wf1.
+- by rewrite e /= andb_false_r in wf1.
+- by rewrite e /= andb_false_r in wf1.
+Qed.
+
+Definition count t t' :=
+  SMS.count PreTerm.inv_aux
+    (unfold_term t) (PreTerm.factors (unfold_term t')).
+
+Lemma count_inj t1 t2 :
+  (∀ x, negb (is_mul x) → count x t1 = count x t2) →
   t1 = t2.
 Proof.
-move=> ecount; apply: unfold_term_inj.
-apply: (PreTerm.count_factors_inj _ _ (wf_unfold_term t1) (wf_unfold_term t2)).
-move=> pt Npt wfpt.
-have wfE : unfold_term (fold_term pt) = pt := fold_termK pt wfpt.
-have Nx : negb (is_mul (fold_term pt)) by rewrite is_mul_unfold wfE.
-rewrite -wfE -(count_factors_unfold t1 Nx) -(count_factors_unfold t2 Nx).
-exact: (ecount _ Nx).
+move=> ecount; apply: factors_inj.
+apply: (inj (fmap unfold_term : list _ → _)).
+rewrite !unfold_factors.
+set ts1 := PreTerm.factors (unfold_term t1).
+set ts2 := PreTerm.factors (unfold_term t2).
+have wfs1: PreTerm.wf_factors ts1 by exact: PreTerm.wf_wf_factors.
+have wfs2: PreTerm.wf_factors ts2 by exact: PreTerm.wf_wf_factors.
+have /SMS.to_id <- := PreTerm.wf_factors_sms _ wfs1.
+have /SMS.to_id <- := PreTerm.wf_factors_sms _ wfs2.
+apply: SMS.count_to_eq.
+- move=> t t_ts; apply: PreTerm.inv_auxK; exact: PreTerm.wf_factors_wf t_ts.
+- move=> t t_ts; apply: PreTerm.inv_auxK; exact: PreTerm.wf_factors_wf t_ts.
+move=> t t_ts.
+have [t' t_t'] : ∃ t', t ∈ PreTerm.factors (unfold_term t').
+  case/elem_of_app: t_ts=> ?; eauto.
+have wf_t: PreTerm.wf t.
+  apply: PreTerm.wf_factors_wf t_t'.
+  exact: PreTerm.wf_wf_factors.
+have tNm: negb (PreTerm.is_mul t).
+  apply: PreTerm.wf_factors_Nmul t_t'.
+  exact: PreTerm.wf_wf_factors.
+rewrite -[t]PreTerm.normalize_wf // -unfold_fold.
+by apply: ecount; rewrite is_mul_unfold fold_termK.
 Qed.
 
-Lemma unfold_base t : unfold_term (base t) = PreTerm.base (unfold_term t).
+Lemma count_TMulN t ts :
+  count t (TMulN ts) = foldr Z.add 0%Z (count t <$> ts).
 Proof.
-by rewrite /base unfold_fold
-  (PreTerm.normalize_wf _ (PreTerm.wf_base _ (wf_unfold_term t))).
+rewrite /count unfold_TMulN /PreTerm.mul PreTerm.mul_auxK; last first.
+  apply: PreTerm.wf_normalize_factors.
+  by apply/Forall_fmap/list.Forall_forall=> ?? /=.
+rewrite /PreTerm.normalize_factors list_fmap_bind SMS.count_to; last first.
+- move=> t0 /list_elem_of_bind [t1 [] /= t0_t1 t1_ts].
+  apply: PreTerm.inv_auxK.
+  apply: PreTerm.wf_factors_wf t0_t1.
+  exact: PreTerm.wf_wf_factors.
+- exact: PreTerm.inv_auxK.
+by elim: ts => //= t0 ts IH; rewrite SMS.count_app IH.
 Qed.
 
-Lemma unfold_exps t :
-  unfold_term <$> exps t = PreTerm.exps (unfold_term t).
+Lemma TInvE t : TInv t = TMulN (TInv <$> factors t).
 Proof.
-rewrite /exps fmap_fold_termK //.
-exact: (PreTerm.wf_exps _ (wf_unfold_term t)).
+apply: unfold_term_inj; rewrite unfold_TMulN unfold_TInv.
+rewrite -list_fmap_compose.
+have ->: unfold_term ∘ TInv <$> factors t =
+         PreTerm.inv_aux ∘ unfold_term <$> factors t.
+  apply/Forall_fmap_ext/list.Forall_forall.
+  move=> t0 t0_in /=; rewrite unfold_TInv PreTerm.inv_Nmul //.
+  have {}t0_in: unfold_term t0 ∈ PreTerm.factors (unfold_term t).
+    by rewrite -unfold_factors; apply/list_elem_of_fmap; eauto.
+  apply: PreTerm.wf_factors_Nmul t0_in.
+  exact: PreTerm.wf_wf_factors.
+rewrite list_fmap_compose unfold_factors /PreTerm.inv.
+case: (unfold_term t) (wf_unfold_term t) => //=.
+case => //= {}t /andb_True [] /andb_True [] tNV tNM wf_t.
+by rewrite PreTerm.mul1.
 Qed.
 
-Lemma factors_one : factors (TMulN []) = [].
+Lemma factors_Nmul t : negb (is_mul t) → factors t = [t].
 Proof.
-have /list_fmap_eq_inj :
-    unfold_term <$> factors (TMulN []) = unfold_term <$> [] => //.
-by rewrite unfold_factors unfold_TMulN.
+rewrite is_mul_unfold => tNm.
+apply: (inj (fmap unfold_term : list _ → _)).
+by rewrite /= unfold_factors PreTerm.factors_Nmul.
 Qed.
 
-Lemma map_unfold_Nmul ts :
-  Forall (fun pt => negb (PreTerm.is_mul pt)) (unfold_term <$> ts) <->
-  Forall (fun t => negb (is_mul t)) ts.
+Lemma factorsK t : TMulN (factors t) = t.
 Proof.
-rewrite Forall_fmap; apply: Forall_iff => t; by rewrite is_mul_unfold.
+apply: unfold_term_inj; rewrite unfold_TMulN unfold_factors.
+rewrite /PreTerm.mul PreTerm.normalize_factors_wf_factors.
+- by rewrite PreTerm.factorsK.
+- exact: PreTerm.wf_wf_factors.
 Qed.
 
-Lemma factors_inj t1 t2 : factors t1 = factors t2 -> t1 = t2.
+Lemma factors_TMulN0 : factors (TMulN []) = [].
+Proof. by rewrite !unlock /=. Qed.
+
+Lemma count_TInv t t' : count t (TInv t') = (- count t t')%Z.
 Proof.
-move=> efactors; apply: unfold_term_inj.
-apply: PreTerm.factors_inj.
-- exact: wf_unfold_term.
-- exact: wf_unfold_term.
-by rewrite -!unfold_factors efactors.
+rewrite TInvE count_TMulN -list_fmap_compose.
+have ->: count t ∘ TInv <$> factors t' =
+         (λ t0, - count t t0)%Z <$> factors t'.
+  apply/Forall_fmap_ext/list.Forall_forall=> t0 t0_in /=.
+  rewrite -(list_elem_of_fmap_inj unfold_term) unfold_factors in t0_in.
+  have t0_Nmul: negb (PreTerm.is_mul (unfold_term t0)).
+    apply: PreTerm.wf_factors_Nmul t0_in.
+    exact: PreTerm.wf_wf_factors.
+  have t0V_Nmul: negb (PreTerm.is_mul (PreTerm.inv_aux (unfold_term t0))).
+    case: (unfold_term t0) (wf_unfold_term t0) t0_Nmul {t0_in} => //=.
+    by case => //= ? /andb_True [] /andb_True [].
+  rewrite /count unfold_TInv PreTerm.inv_Nmul //.
+  rewrite PreTerm.factors_Nmul // PreTerm.factors_Nmul //.
+  rewrite -SMS.count_fmap_i //.
+  - exact: PreTerm.inv_auxK.
+  - move=> ? /list_elem_of_singleton ->.
+    exact: PreTerm.inv_auxK.
+rewrite -[t' in RHS]factorsK count_TMulN.
+elim: {t'} (factors t') => //= t' ts ->; rewrite /fmap; lia.
 Qed.
 
-Lemma factors_atomic t : negb (is_mul t) -> factors t = [t].
+Lemma count_TMulN_app t ts1 ts2 :
+  count t (TMulN (ts1 ++ ts2)) =
+  (count t (TMulN ts1) + count t (TMulN ts2))%Z.
 Proof.
-move=> Nt; apply: (inj (fmap unfold_term)); rewrite unfold_factors.
-have Nt' : negb (PreTerm.is_mul (unfold_term t)) by rewrite -is_mul_unfold.
-by rewrite (PreTerm.factorsN _ Nt').
+rewrite !count_TMulN.
+elim: ts1 => //= t' ts1 ->; rewrite /fmap; lia.
 Qed.
 
-Lemma count_factors_TMulN_concat x ts :
-  negb (is_mul x) ->
-  SMS.count TInv x (factors (TMulN ts)) =
-  SMS.count TInv x (concat (factors <$> ts)).
+Lemma base_idem pt : base (base pt) = base pt.
 Proof.
-move=> Nx; elim: ts => [|u ts IH].
-- by rewrite factors_one.
-- rewrite fmap_cons concat_cons (count_factors_TMulN x u ts Nx) IH.
-  by rewrite (SMS.count_app TInv x (factors u) (concat (factors <$> ts))).
+apply: unfold_term_inj; rewrite !unfold_base.
+rewrite PreTerm.base_expN //; exact: PreTerm.base_Nexp.
 Qed.
 
-Definition atomic (ts : list term) : Prop := Forall (fun t => negb (is_mul t)) ts.
-
-Lemma atomic_unfold ts :
-  atomic ts -> Forall (fun pt => negb (PreTerm.is_mul pt)) (unfold_term <$> ts).
-Proof. rewrite /atomic; exact: (proj2 (map_unfold_Nmul ts)). Qed.
-
-Lemma atom_factors t : atomic (factors t).
+Lemma TMulN1 t : TMulN [t] = t.
 Proof.
-apply/Forall_forall => x x_t; rewrite is_mul_unfold.
-have /list.Forall_forall H := PreTerm.Nmul_factors _ (wf_unfold_term t).
-apply: H; rewrite -unfold_factors; apply: list_elem_of_fmap_2; exact: x_t.
+by apply: unfold_term_inj; rewrite unfold_TMulN /= PreTerm.mul1.
 Qed.
 
-Lemma fmap_TInv_fold_term pts :
-  Forall PreTerm.wf pts ->
-  Forall (fun pt => negb (PreTerm.is_mul pt)) pts ->
-  TInv <$> (fold_term <$> pts) = fold_term <$> (PreTerm.inv_aux <$> pts).
+Lemma TMulN_unit_r t : TMulN [t; TMulN []] = t.
 Proof.
-elim: pts => [//|pt pts IH] /Forall_cons [Wpt wfs] /Forall_cons [Nmpt Nms].
-rewrite !fmap_cons (IH wfs Nms); congr cons.
-apply: unfold_term_inj.
-by rewrite unfold_TInv (fold_termK pt Wpt)
-           (fold_termK (PreTerm.inv_aux pt) (PreTerm.wf_inv_aux pt Wpt Nmpt))
-           (PreTerm.inv_Nmul pt Nmpt).
+apply: count_inj=> t0 ?; rewrite count_TMulN /= count_TMulN /=; lia.
+Qed.
+
+Lemma base_Nexp t : negb (is_exp (base t)).
+Proof. rewrite is_exp_unfold unfold_base; exact: PreTerm.base_Nexp. Qed.
+
+Lemma expo_expN t : negb (is_exp t) → expo t = TMulN [].
+Proof.
+rewrite is_exp_unfold => tNx; apply: unfold_term_inj.
+rewrite unfold_expo unfold_TMulN /=.
+exact: PreTerm.expo_expN.
+Qed.
+
+Lemma base_expN t : negb (is_exp t) → base t = t.
+Proof.
+rewrite is_exp_unfold => tNx; apply: unfold_term_inj.
+rewrite unfold_base; exact: PreTerm.base_expN.
+Qed.
+
+Lemma TExpE b e : TExp b e = TExp (base b) (TMulN [expo b; e]).
+Proof.
+apply: unfold_term_inj; rewrite !unfold_TExp !unfold_base !unfold_TMulN /=.
+rewrite unfold_expo /PreTerm.exp.
+rewrite [PreTerm.expo (PreTerm.base _)]PreTerm.expo_expN //.
+- rewrite -!unfold_base base_idem PreTerm.mul_unit_l PreTerm.mul1 //.
+  apply: PreTerm.wf_mul; rewrite Forall_cons_iff Forall_singleton.
+  split => //; exact: PreTerm.wf_expo.
+- exact: PreTerm.base_Nexp.
+Qed.
+
+Lemma TExp_base_expo t : TExp (base t) (expo t) = t.
+Proof.
+apply: unfold_term_inj; rewrite unfold_TExp unfold_base unfold_expo.
+rewrite /PreTerm.exp -!unfold_base -unfold_expo base_idem.
+rewrite expo_expN; last exact: base_Nexp.
+rewrite unfold_TMulN /= PreTerm.mul_unit_l -unfold_expo.
+rewrite -(unfold_TMulN [expo t]) TMulN1 unfold_base unfold_expo.
+case: t; case => //=; case=> //= t1 t2.
+rewrite !andb_True; case=> [] [] [] wf1 t1Nx wf2 /bool_decide_spec t2N1.
+by rewrite /PreTerm.exp_aux bool_decide_eq_false_2.
+Qed.
+
+Lemma base_TExp b e : base (TExp b e) = base b.
+Proof.
+apply: unfold_term_inj; rewrite !unfold_base unfold_TExp.
+rewrite /base // /PreTerm.exp /PreTerm.exp_aux -/(PreTerm.base _).
+case_bool_decide as H => //.
+by rewrite -!unfold_base base_idem.
+Qed.
+
+Lemma expo_TExp b e : expo (TExp b e) = TMulN [expo b; e].
+Proof.
+apply: unfold_term_inj; rewrite !unfold_expo unfold_TExp unfold_TMulN /=.
+rewrite unfold_expo /PreTerm.exp /PreTerm.exp_aux.
+case_bool_decide as H => //.
+rewrite H -unfold_base -unfold_expo expo_expN ?unfold_TMulN //=.
+exact: base_Nexp.
+Qed.
+
+Lemma TExp_unit b : TExp b (TMulN []) = b.
+Proof.
+rewrite -[LHS]TExp_base_expo -[RHS]TExp_base_expo.
+by rewrite base_TExp expo_TExp TMulN_unit_r.
+Qed.
+
+Definition exps pt := factors (expo pt).
+
+Instance perm_TMulN : Proper ((≡ₚ) ==> (=)) TMulN.
+Proof.
+move=> ts1 ts2 peq; apply: count_inj => t tNm.
+rewrite !count_TMulN; apply: foldr_permutation_proper.
+- lia.
+- by rewrite peq.
+Qed.
+
+Lemma TMulN_cat ts1 ts2 : TMulN (TMulN ts1 :: ts2) = TMulN (ts1 ++ ts2).
+Proof.
+apply: count_inj => t tNm.
+by rewrite (count_TMulN_app _ [TMulN ts1]) count_TMulN_app TMulN1.
+Qed.
+
+Lemma TExpA b e1 e2 : TExp (TExp b e1) e2 = TExp b (TMulN [e1; e2]).
+Proof.
+rewrite -[LHS]TExp_base_expo -[RHS]TExp_base_expo.
+rewrite !base_TExp !expo_TExp TMulN_cat /=.
+rewrite [in RHS]Permutation_swap TMulN_cat /=.
+by rewrite -[[e1; e2; expo b]]/([e1; e2] ++ [expo b]) Permutation_app_comm.
+Qed.
+
+Lemma TMulN_inv_r t : TMulN [TInv t; t] = TMulN [].
+Proof.
+apply: count_inj=> t0 t0Nm; rewrite !count_TMulN /=.
+rewrite count_TInv; lia.
+Qed.
+
+Lemma TMulN_eq_unit ts : TMulN ts = TMulN [] ↔ factors (TMulN ts) = [].
+Proof.
+split.
+- move=> /(f_equal factors) => ->.
+  apply: (inj (fmap unfold_term : list _ → _)).
+  by rewrite unfold_factors /= unfold_TMulN.
+- by move=> <-; rewrite factorsK.
+Qed.
+
+Lemma TInv_Nid t : negb (is_mul t) → TInv t ≠ t.
+Proof.
+move=> tNm e.
+have {}e : is_inv t = negb (is_inv t) by rewrite -{1}e is_inv_TInv.
+by case: is_inv e.
+Qed.
+
+Lemma TInvK t : TInv (TInv t) = t.
+Proof. apply: count_inj=> t0 _; rewrite !count_TInv; lia. Qed.
+
+Definition invs_canceled (ts : list term) : Prop :=
+  ∀ t, t ∈ ts → TInv t ∉ ts ∧ negb (is_mul t).
+
+Lemma invs_canceled0 : invs_canceled [].
+Proof. by move=> ? /elem_of_nil. Qed.
+
+Lemma invs_canceled_cons t ts :
+  invs_canceled (t :: ts) ↔
+  TInv t ∉ ts ∧ negb (is_mul t) ∧ invs_canceled ts.
+Proof.
+split.
+- move=> ic.
+  have /ic [Vnin tNm] : t ∈ t :: ts by rewrite elem_of_cons; eauto.
+  do 2?split => //.
+  + by move=> contra; apply: Vnin; apply/elem_of_cons; eauto.
+  + move=> t0 t0_in.
+    have /ic [V0nin t0Nm] : t0 ∈ t :: ts by rewrite elem_of_cons; eauto.
+    by split=> // contra; apply: V0nin; apply/elem_of_cons; eauto.
+- case=> Vnin [] tNm ic t0 /elem_of_cons [->|t0_in].
+  + split=> // /elem_of_cons [e|//].
+    exact: TInv_Nid.
+  + have /ic [V0nin t0Nm] := t0_in.
+    split => // /elem_of_cons [e|//].
+    rewrite -e TInvK in Vnin; tauto.
+Qed.
+
+Lemma wf_factors_invs_canceled (ts : list _) :
+  PreTerm.wf_factors ts →
+  invs_canceled (fold_term <$> ts).
+Proof.
+case/andb_True=> [] /forallb_True/Forall_forall wfts sms.
+move=> _ /list_elem_of_fmap [t [] -> t_ts].
+have /andb_True [wft tNm] := wfts _ t_ts.
+rewrite is_mul_unfold fold_termK //; split => //.
+rewrite -(list_elem_of_fmap_inj unfold_term) unfold_TInv fold_termK //.
+rewrite PreTerm.inv_Nmul //.
+have -> : unfold_term <$> (fold_term <$> ts) = ts.
+  rewrite -[RHS]list_fmap_id -list_fmap_compose; apply/Forall_fmap_ext.
+  apply/Forall_forall=> t0 /wfts/andb_True [wft0 ?].
+  by rewrite /= fold_termK.
+by move/SMS.wf_no_pairs/(_ _ t_ts) in sms.
 Qed.
 
 Lemma term_rect (T : term -> Type)
@@ -545,8 +712,7 @@ Lemma term_rect (T : term -> Type)
                    t2 ≠ TMulN [] ->
         T (TExp t1 t2))
   (H9 : forall ts, foldr (fun t R => T t * R)%type unit ts ->
-                   atomic ts ->
-                   (forall t', t' ∈ ts -> TInv t' ∉ ts) ->
+                   invs_canceled ts →
                    length ts ≠ 1 ->
         T (TMulN ts)) :
   forall t, T t.
@@ -571,25 +737,18 @@ elim: (unfold_term t) (wf_unfold_term t)=>
     * by rewrite is_exp_unfold (fold_termK _ w1).
     * have E0 : TMulN [] = fold_term (PreTerm.PTMul []) by rewrite fold_termE.
       rewrite E0 => Heq; apply: pt2N.
-      by move: (f_equal unfold_term Heq);
-        rewrite (fold_termK _ w2) (fold_termK _ PreTerm.wf_nil) => ->.
-- have [wfts [Nmts [sms lenN1]]] := PreTerm.wf_Mul_inv _ wfpt.
-  rewrite fold_termE; apply: H9.
-  + elim: ts IHts wfts {wfpt Nmts sms lenN1} => [//|pt ts' IH] /=.
+      move/(f_equal unfold_term): Heq.
+      by rewrite fold_termK // fold_termK.
+- rewrite fold_termE.
+  have [wff tsN1]: PreTerm.wf_factors ts ∧ length ts ≠ 1.
+    by rewrite /= andb_True bool_decide_spec in wfpt; case: wfpt.
+  apply: H9.
+  + have {}wfts: Forall PreTerm.wf ts.
+      by apply/list.Forall_forall => ?; apply: PreTerm.wf_factors_wf.
+    elim: ts IHts wfts {wfpt wff tsN1} => [//|pt ts' IH] /=.
     move=> [IHpt IHts'] /Forall_cons [w ws].
     by split; [exact: (IHpt w)|exact: (IH IHts' ws)].
-  + move/list.Forall_forall in wfts.
-    move/list.Forall_forall in Nmts.
-    apply/Forall_fmap/list.Forall_forall => t t_ts /=.
-    rewrite /= is_mul_unfold fold_termK //; eauto.
-  + move=> _ /list_elem_of_fmap [t [] -> t_ts] tV_ts.
-    move/SMS.wf_no_pairs in sms; apply: sms (t_ts) _.
-    rewrite -[ts]fmap_fold_termK //; apply/list_elem_of_fmap.
-    exists (TInv (fold_term t)); split => //.
-    have wft: PreTerm.wf t by move/list.Forall_forall: wfts; exact.
-    rewrite unfold_TInv_Nmul ?fold_termK //.
-    rewrite is_mul_unfold // fold_termK //.
-    move/list.Forall_forall: Nmts; exact.
+  + exact: wf_factors_invs_canceled.
   + by rewrite length_fmap.
 Qed.
 
